refinedVST/lithium/solvers.v
@@ -242,7 +242,7 @@ Ltac reduce_closed_Z :=
 
 
 Ltac solve_goal :=
-  simpl;
+  simpl in *;
   try fast_done;
   solve_goal_prepare_hook;
   normalize_and_simpl_goal;
